Checkpoint before changing Layer2

src/Confidentiality.v
@@ -1,116 +1,7 @@
-Require Import Primitives.
+Require Import BaseTypes Memx Disk CommonAutomation.
 Require Import Simulation.
-Close Scope pred_scope.
 
-Lemma deterministic_prog:
-  forall T (p: prog T) u o s d ret1 ret2 tr1 tr2,
-    exec u o s d p ret1 tr1 ->
-    exec u o s d p ret2 tr2 ->
-    ret1 = ret2 /\ tr1 = tr2.
-Proof.
-  induction p; simpl; intros;
-    inv_exec_perm; cleanup;
-      inv_exec_perm; cleanup; eauto.
-  intuition.
-  intuition.
-
-  specialize IHp with (1:= H0)(2:=H1); cleanup.
-  specialize H with (1:= H2)(2:=H3); cleanup.
-  eauto.
-  
-  destruct H0; cleanup.
-  specialize IHp with (1:= H0)(2:=H1); cleanup.
-  specialize IHp with (1:= H0)(2:=H1); cleanup.
-  specialize H with (1:= H2)(2:=H3); cleanup.
-
-  destruct H1; cleanup.
-  specialize IHp with (1:= H0)(2:=H1); cleanup.
-  specialize IHp with (1:= H0)(2:=H1); cleanup.
-  specialize H with (1:= H2)(2:=H3); cleanup.
-
-  destruct H0; cleanup; destruct H1; cleanup.
-  specialize IHp with (1:= H0)(2:=H1); cleanup; eauto.
-  
-  specialize IHp with (1:= H0)(2:=H1); cleanup.
-
-  specialize IHp with (1:= H0)(2:=H1); cleanup.
-
-  specialize IHp with (1:= H0)(2:=H1); cleanup.
-  specialize H with (1:= H2)(2:=H3); cleanup.
-  eauto.
-Qed.
-
-Definition data_except u (d: disk):=
-  fun a =>
-    match d a with
-    | None => d a
-    | Some vs =>
-      let value := (fst vs) in
-      if can_access_dec u (fst value) then
-        if permission_dec (fst value) Public then
-          d a
-        else
-          None
-      else
-        d a
-    end.
-
-Definition data_except_store u (s: store):=
-  fun a =>
-    match s a with
-    | None => s a
-    | Some value =>
-      if can_access_dec u (fst value) then
-        if permission_dec (fst value) Public then
-          s a
-        else
-          None
-      else
-        s a
-    end.
-
-Definition equivalent_except u (d1 d2: disk):=
-  forall a,
-    (d1 a = None /\ d2 a = None) \/
-    (exists vs1 vs2,
-        d1 a = Some vs1 /\ d2 a = Some vs2 /\
-        fst (fst vs1) =  fst (fst vs2) /\
-        ((fst (fst vs1) = Public \/ ~can_access u (fst (fst vs1))) ->
-         snd (fst vs1) = snd (fst vs2)))%type.
-
-Definition equivalent_except_store u (s1 s2: store):=
-  forall a,
-    (s1 a = None /\ s2 a = None) \/
-    (exists v1 v2,
-        s1 a = Some v1 /\ s2 a = Some v2 /\
-        fst v1 =  fst v2 /\
-        ((fst v1 = Public \/ ~can_access u (fst v1)) ->
-         snd v1 = snd v2))%type.
-
-Definition data_of def u (d: disk):=
-  fun a =>
-    match d a with
-    | None => None
-    | Some vs =>
-      let value := (fst vs) in
-      if can_access_dec u (fst value) then
-        d a
-      else
-        Some def
-    end.
-
-Definition data_of_store def u (s: store):=
-  fun a =>
-    match s a with
-    | None => None
-    | Some value =>
-      if can_access_dec u (fst value) then
-        s a
-      else
-        Some def
-    end.
-
-Definition equivalent_for u (d1 d2: disk):=
+Definition equivalent_for_fst {A AEQ V} u (d1 d2: @mem A AEQ ((permission * V) * list (permission * V))):=
   forall a,
     (d1 a = None /\ d2 a = None) \/
     (exists vs1 vs2,
@@ -118,128 +9,78 @@ Definition equivalent_for u (d1 d2: disk):=
         (can_access u (fst (fst vs1)) ->
         fst vs1 =  fst vs2))%type.
 
-Definition equivalent_for_store u (s1 s2: store):=
+Definition equivalent_for {A AEQ V} u (d1 d2: @mem A AEQ (permission * V)):=
   forall a,
-    (s1 a = None /\ s2 a = None) \/
+    (d1 a = None /\ d2 a = None) \/
     (exists v1 v2,
-        s1 a = Some v1 /\ s2 a = Some v2 /\
+        d1 a = Some v1 /\ d2 a = Some v2 /\
         (can_access u (fst v1) ->
         v1 = v2))%type.
 
-Lemma data_of_implies_equivalent_for:
-  forall u (d1 d2: disk),
-    (forall def a, data_of def u d1 a = data_of def u d2 a) ->
-    equivalent_for u d1 d2.
-Proof. Abort.
 
-Lemma hoare_triple_to_trace_ok:
-  forall T (p: prog T) pre post crash,
-    hoare_triple pre p post crash ->
-    (forall u o s d,
-       pre u o s d ->
-       (forall ret tr,
-          exec u o d s p ret tr ->
-          trace_ok tr)).
-Proof.
-  unfold hoare_triple; intros.
-  specialize H with (1:= H0) (2:= H1); cleanup; eauto.
-Qed.
-
-Definition ret_noninterference {T} (p: prog T) :=
-  forall u o d1 d2 s1 s2 ret1 tr,
-    exec u o d1 s1 p ret1 tr ->
-    equivalent_for u d1 d2 ->
-    equivalent_for_store u s1 s2 ->
-    trace_ok tr ->
-    (exists ret2,
-        exec u o d2 s2 p ret2 tr /\
-     (exists o' d1' s1' d2' s2',
-         ((exists r, ret1 = Finished o' d1' s1' r /\ ret2 = Finished o' d2' s2' r) \/
-          (ret1 = Crashed _ o' d1' s1' /\ ret2 = Crashed _ o' d2' s2')) /\
-         equivalent_for u d1' d2' /\
-         equivalent_for_store u s1' s2'))%type.
-
-Lemma equivalent_for_store_none:
-  forall u s1 s2 h,
-    equivalent_for_store u s1 s2 ->
+Lemma equivalent_for_none:
+  forall A AEQ V u s1 s2 h,
+    @equivalent_for A AEQ V u s1 s2 ->
     s1 h = None ->
     s2 h = None.
 Proof.
-  unfold equivalent_for_store; simpl; intros.
-  specialize (H h); destruct H; cleanup; eauto.
+  unfold equivalent_for; simpl; intros.
+  specialize (H h); destruct H; intuition eauto.
+  do 2 destruct H; intuition.
+  rewrite H0 in H1; inversion H1.
 Qed.
 
-Lemma equivalent_for_read:
-      forall u d1 d2 a v,
-        equivalent_for u d1 d2 ->
+Lemma equivalent_for_fst_read:
+      forall u (d1 d2: disk) a v,
+        @equivalent_for_fst _ addr_dec _ u d1 d2 ->
         read d1 a = Some v ->
         exists v', read d2 a = Some v' /\
               (can_access u (fst v) ->
               v = v').
 Proof.
   unfold read, equivalent_for; simpl; intros.
-  specialize (H a); destruct H; cleanup; eauto.
+  specialize (H a); destruct H; intuition eauto.
+  rewrite H1 in H0; inversion H0.
+  do 2 destruct H; intuition eauto.
+  rewrite H1 in H0; inversion H0; subst.
+  eexists; rewrite H; eauto.
 Qed.
 
-Lemma equivalent_for_store_upd_store:
+Lemma equivalent_for_upd_store:
   forall u s1 s2 h v x,
-    equivalent_for_store u s1 s2 ->
+    equivalent_for u s1 s2 ->
     (can_access u (fst v) -> v = x) ->
-    equivalent_for_store u (upd_store s1 h v) (upd_store s2 h x).
+    equivalent_for u (upd_store s1 h v) (upd_store s2 h x).
 Proof.
-  unfold equivalent_for_store, upd_store; simpl; intros.
+  unfold equivalent_for, upd_store; simpl; intros.
   destruct (handle_dec a h); subst.
   - repeat rewrite upd_eq; eauto.
     right; eauto.
   - repeat rewrite upd_ne; eauto.
 Qed.
 
-Lemma not_none_iff_some:
-  forall T (exp: option T),
-    exp <> None <->
-    exists t, exp = Some t.
-Proof.
-  intros; split; intros; destruct exp;
-  intuition eauto; cleanup.
-Qed.
-
-Lemma equivalent_for_store_some:
-  forall u s1 s2 h v,
-    equivalent_for_store u s1 s2 ->
+Lemma equivalent_for_some:
+  forall A AEQ V u s1 s2 h v,
+    @equivalent_for A AEQ V u s1 s2 ->
     s1 h = Some v ->
     exists v', s2 h = Some v' /\
           (can_access u (fst v) -> v = v').
 Proof.
-  unfold equivalent_for_store; simpl; intros.
-  specialize (H h); destruct H; cleanup; eauto.
+  unfold equivalent_for; simpl; intros.
+  specialize (H h); destruct H; intuition eauto.
+  rewrite H1 in H0; inversion H0.
+  do 2 destruct H; intuition eauto.
+  rewrite H1 in H0; inversion H0; subst.
+  eexists; rewrite H; eauto.
 Qed.
 
-Tactic Notation "eapply_fresh" constr(thm) "in" hyp(H) :=
-  let Hx := fresh "Hx" in eapply thm in H as Hx.
-
-Tactic Notation "destruct_fresh" constr(term) :=
-  let D := fresh "D" in destruct term eqn:D.
-
-Tactic Notation "assert_fresh" constr(ass) :=
-  let A := fresh "A" in assert ass as A.
-
-Lemma trace_ok_app_split:
-  forall tr tr',
-    trace_ok (tr++tr') ->
-    trace_ok tr /\ trace_ok tr'.
-Proof.
-  induction tr; simpl; intros; eauto.
-  destruct a; simpl in *; cleanup; intuition eauto.
-  all: specialize IHtr with (1:= H0); cleanup; eauto.
-Qed.
-
-Lemma equivalent_for_write:
+Lemma equivalent_for_fst_write:
   forall u d1 d2 a v v',
-    equivalent_for u d1 d2 ->
+    equivalent_for_fst u d1 d2 ->
     (can_access u (fst v) -> v = v') ->
-    equivalent_for u (write d1 a v) (write d2 a v').
+    @equivalent_for_fst _ addr_dec _ u (write d1 a v) (write d2 a v').
 Proof.
-  unfold equivalent_for, write, upd_disk; intros.
+  unfold equivalent_for_fst, write, upd_disk; intros.
   specialize (H a0).
   destruct (addr_dec a a0); subst.
   
@@ -255,6 +96,21 @@ Proof.
   repeat rewrite upd_ne; eauto.
 Qed.
 
+Lemma not_none_iff_some:
+  forall T (exp: option T),
+    exp <> None <->
+    exists t, exp = Some t.
+Proof.
+  intros; split; intros; destruct exp;
+    intuition eauto; inversion H0.
+  destruct H; inversion H.
+Qed.
+
+
+
+
+(*
+
 Theorem trace_ok_to_ret_noninterference:
   forall T (p: prog T),
     ret_noninterference p.
@@ -262,12 +118,12 @@ Proof.
   unfold ret_noninterference; induction p; simpl in *;
   intros; try specialize H with (1:=H0) as Hx; inv_exec_perm.
   { (*Read*)
-    eapply_fresh equivalent_for_read in H0 ; eauto; cleanup.
+    eapply_fresh equivalent_for_fst_read in H0 ; eauto; cleanup.
     eexists; intuition eauto.
     econstructor; eauto.
-    eapply equivalent_for_store_none; eauto.
+    eapply equivalent_for_none; eauto.
     do 5 eexists; intuition eauto.
-    eapply equivalent_for_store_upd_store; eauto.
+    eapply equivalent_for_upd_store; eauto.
   }
   { (*Read Crash*)
     eexists; intuition eauto.
@@ -276,13 +132,13 @@ Proof.
   }
   { (*Write*)
     apply not_none_iff_some in H12; cleanup.
-    eapply_fresh equivalent_for_read in H0; eauto; cleanup.
-    eapply_fresh equivalent_for_store_some in H1; eauto; cleanup.
+    eapply_fresh equivalent_for_fst_read in H0; eauto; cleanup.
+    eapply_fresh equivalent_for_some in H1; eauto; cleanup.
     eexists; intuition eauto.
     econstructor; eauto.
     eapply not_none_iff_some; eauto.
     do 5 eexists; intuition eauto.
-    eapply equivalent_for_write; eauto.
+    eapply equivalent_for_fst_write; eauto.
   }
   { (*Write Crash*)
     eexists; intuition eauto.
@@ -307,9 +163,9 @@ Proof.
   { (*Seal*)
     eexists; intuition eauto.
     econstructor; eauto.
-    eapply equivalent_for_store_none; eauto.
+    eapply equivalent_for_none; eauto.
     do 5 eexists; intuition eauto.
-    eapply equivalent_for_store_upd_store; eauto.
+    eapply equivalent_for_upd_store; eauto.
   }
   { (*Auth Crash*)
     eexists; intuition eauto.
@@ -320,7 +176,7 @@ Proof.
     unfold trace_ok in H2; simpl in *; cleanup.
     eexists; intuition eauto.
     econstructor; eauto.
-    eapply equivalent_for_store_some in H1; eauto; cleanup.
+    eapply equivalent_for_some in H1; eauto; cleanup.
     intuition; cleanup; eauto.
     do 5 eexists; intuition eauto.
   }
@@ -373,13 +229,13 @@ Qed.
 Definition ret_noninterference_precondition {T} (pre: precond) (p: prog T) :=
   forall u o d1 d2 s1 s2 o1' d1' s1' r1 tr1,
     exec u o d1 s1 p (Finished o1' d1' s1' r1) tr1 ->
-    equivalent_for u d1 d2 ->
-    equivalent_for_store u s1 s2 ->
+    equivalent_for_fst u d1 d2 ->
+    equivalent_for u s1 s2 ->
     pre u o s1 d1 ->
     (exists o2' d2' s2' r2 tr2,
       exec u o d2 s2 p (Finished o2' d2' s2' r2) tr2 /\
-      equivalent_for u d1' d2' /\
-      equivalent_for_store u s1' s2' /\
+      @equivalent_for_fst _ addr_dec _ u d1' d2' /\
+      @equivalent_for _ handle_dec _ u s1' s2' /\
       tr1 = tr2 /\
       o1' = o2' /\
       r1 = r2)%type.
@@ -392,20 +248,20 @@ Proof.
   unfold ret_noninterference_precondition; induction p; simpl in *;
   intros; try specialize H with (1:=H0) as Hx; inv_exec_perm.
   { (*Read*)
-    eapply_fresh equivalent_for_read in H1 ; eauto; cleanup.
+    eapply_fresh equivalent_for_fst_read in H1 ; eauto; cleanup.
     do 5 eexists; intuition eauto.
     econstructor; eauto.
-    eapply equivalent_for_store_none; eauto.
-    eapply equivalent_for_store_upd_store; eauto.
+    eapply equivalent_for_none; eauto.
+    eapply equivalent_for_upd_store; eauto.
   }
   { (*Write*)
     apply not_none_iff_some in H17; cleanup.
-    eapply_fresh equivalent_for_read in H1; eauto; cleanup.
-    eapply_fresh equivalent_for_store_some in H2; eauto; cleanup.
+    eapply_fresh equivalent_for_fst_read in H1; eauto; cleanup.
+    eapply_fresh equivalent_for_some in H2; eauto; cleanup.
     do 5 eexists; intuition eauto.
     econstructor; eauto.
     eapply not_none_iff_some; eauto.
-    eapply equivalent_for_write; eauto.
+    eapply equivalent_for_fst_write; eauto.
   }
   { (*Auth Success*)
     do 5 eexists; intuition eauto.
@@ -418,8 +274,8 @@ Proof.
   { (*Seal*)
     do 5 eexists; intuition eauto.
     econstructor; eauto.
-    eapply equivalent_for_store_none; eauto.
-    eapply equivalent_for_store_upd_store; eauto.
+    eapply equivalent_for_none; eauto.
+    eapply equivalent_for_upd_store; eauto.
   }
   { (*Unseal*)
     eapply hoare_triple_to_trace_ok in H3; eauto.
@@ -427,7 +283,7 @@ Proof.
     unfold trace_ok in H3; simpl in *; cleanup.
     do 5 eexists; intuition eauto.
     econstructor; eauto.
-    eapply equivalent_for_store_some in H2; eauto; cleanup.
+    eapply equivalent_for_some in H2; eauto; cleanup.
     intuition; cleanup; eauto.
   }
   { (*Ret*)
@@ -443,4 +299,6 @@ eapply trace_ok_to_ret_noninterference in H1; eauto.
     econstructor; eauto.
   }
 Qed.
+*)
+
 *)
