src/Prog.v
@@ -1,9 +1,16 @@
-Require Import List BaseTypes Memx Disk.
+Require Import List BaseTypes Memx CommonAutomation.
+Require Import Confidentiality Disk Simulation.
 Import ListNotations.
 
 Set Implicit Arguments.
 
 Section Prog.
+
+  Definition state := (user * oracle * disk * store)%type.
+  Definition get_user (st: state) := fst (fst (fst st)).
+  Definition get_oracle (st: state) := snd (fst (fst st)).
+  Definition get_disk (st: state) := snd (fst st).
+  Definition get_store (st: state) := snd st.
   
   Inductive prog : Type -> Type :=
   | Read : addr -> prog handle
@@ -16,98 +23,206 @@ Section Prog.
   | Ret : forall T, T -> prog T
   | Bind : forall T T', prog T -> (T -> prog T') -> prog T'.
 
-  Inductive result : Type -> Type :=
-  | Finished : forall T, oracle -> disk -> store -> T -> result T
-  | Crashed : forall T, oracle -> disk -> store -> result T.
                                
   Inductive exec :
-    forall T, user -> oracle -> disk -> store -> prog T -> result T -> trace -> Prop :=
+    forall T, state -> prog T -> @Result state T -> trace -> Prop :=
   | ExecRead : 
-      forall u o o' d s a v h,
+      forall st o' a v h,
+        let u := fst (fst (fst st)) in
+        let o := snd (fst (fst st)) in
+        let d := snd (fst st) in
+        let s := snd st in
         o = (Handle h)::o' ->
         s h = None ->
         read d a = Some v ->
-        exec u o d s (Read a) (Finished o' d (upd_store s h v) h) []
+        exec st (Read a) (Finished (u, o', d, (upd_store s h v)) h) []
              
   | ExecWrite :
-      forall u o o' d s a v h,
+      forall st o' a v h,
+        let u := fst (fst (fst st)) in
+        let o := snd (fst (fst st)) in
+        let d := snd (fst st) in
+        let s := snd st in
         o = Cont::o' ->
         s h = Some v ->
         read d a <> None ->
-        exec u o d s (Write a h) (Finished o (write d a v) s tt) []
+        exec st (Write a h) (Finished (u, o, (write d a v), s) tt) []
              
   | ExecAuthSucc :
-      forall u o o' d s p,
+      forall st o' p,
+        let u := fst (fst (fst st)) in
+        let o := snd (fst (fst st)) in
+        let d := snd (fst st) in
+        let s := snd st in
         o = Cont::o' ->
         can_access u p ->
-        exec u o d s (Auth p) (Finished o d s true) []
+        exec st (Auth p) (Finished (u, o, d, s) true) []
 
   | ExecAuthFail :
-      forall u o o' d s p,
+      forall st o' p,
+        let u := fst (fst (fst st)) in
+        let o := snd (fst (fst st)) in
+        let d := snd (fst st) in
+        let s := snd st in
         o = Cont::o' ->
         ~can_access u p ->
-        exec u o d s (Auth p) (Finished o d s false) []
+        exec st (Auth p) (Finished (u, o, d, s) false) []
 
   | ExecSeal :
-      forall u o o' d s p v h,
+      forall st o' p v h,
+        let u := fst (fst (fst st)) in
+        let o := snd (fst (fst st)) in
+        let d := snd (fst st) in
+        let s := snd st in
         o = (Handle h)::o' ->
         s h = None ->
-        exec u o d s (Seal p v) (Finished o' d (upd_store s h (p, v)) h) []
+        exec st (Seal p v) (Finished (u, o', d, (upd_store s h (p, v))) h) []
 
   | ExecUnseal :
-      forall u o o' d s v h,
+      forall st o' v h,
+        let u := fst (fst (fst st)) in
+        let o := snd (fst (fst st)) in
+        let d := snd (fst st) in
+        let s := snd st in
         o = Cont::o' ->
         s h = Some v ->
-        exec u o d s (Unseal h) (Finished o d s (snd v)) [Uns u (fst v)]
+        exec st (Unseal h) (Finished (u, o, d, s) (snd v)) [Uns u (fst v)]
 
   | ExecRet :
-      forall T u o o' d s (v: T),
+      forall st o' T (v: T),
+        let u := fst (fst (fst st)) in
+        let o := snd (fst (fst st)) in
+        let d := snd (fst st) in
+        let s := snd st in
         o = Cont::o' ->
-        exec u o d s (Ret v) (Finished o d s v) []
+        exec st (Ret v) (Finished (u, o, d, s) v) []
 
   | ExecBind :
       forall T T' (p1: prog T) (p2: T -> prog T')
-        u o d s o1 d1 s1 r tr1 ret tr2,
-        exec u o d s p1 (Finished o1 d1 s1 r) tr1 ->
-        exec u o1 d1 s1 (p2 r) ret tr2 ->
-        exec u o d s (Bind p1 p2) ret (tr1++tr2)
+        st st1 r tr1 ret tr2,
+        exec st p1 (Finished st1 r) tr1 ->
+        exec st1 (p2 r) ret tr2 ->
+        exec st (Bind p1 p2) ret (tr1++tr2)
 
   | ExecReadCrash :
-      forall u o d s o' a,
+      forall st o' a,
+        let u := fst (fst (fst st)) in
+        let o := snd (fst (fst st)) in
+        let d := snd (fst st) in
+        let s := snd st in
         o = Crash::o' ->
-        exec u o d s (Read a) (Crashed _ o' d s) []
+        exec st (Read a) (Crashed (u, o', d, s)) []
              
   | ExecWriteCrash :
-      forall u o d s o' a h,
+      forall st o' a h,
+        let u := fst (fst (fst st)) in
+        let o := snd (fst (fst st)) in
+        let d := snd (fst st) in
+        let s := snd st in
         o = Crash::o' ->
-        exec u o d s (Write a h) (Crashed _ o' d s) []
+        exec st (Write a h) (Crashed (u, o', d, s)) []
              
   | ExecAuthCrash :
-      forall u o d s o' p,
+      forall st o' p,
+        let u := fst (fst (fst st)) in
+        let o := snd (fst (fst st)) in
+        let d := snd (fst st) in
+        let s := snd st in
         o = Crash::o' ->
-        exec u o d s (Auth p) (Crashed _ o' d s) []
+        exec st (Auth p) (Crashed (u, o', d, s)) []
              
   | ExecSealCrash :
-      forall u o d s o' p v,
+      forall st o' p v,
+        let u := fst (fst (fst st)) in
+        let o := snd (fst (fst st)) in
+        let d := snd (fst st) in
+        let s := snd st in
         o = Crash::o' ->
-        exec u o d s (Seal p v) (Crashed _ o' d s) []
+        exec st (Seal p v) (Crashed (u, o', d, s)) []
              
   | ExecUnsealCrash :
-      forall u o d s o' h,
+      forall st o' h,
+        let u := fst (fst (fst st)) in
+        let o := snd (fst (fst st)) in
+        let d := snd (fst st) in
+        let s := snd st in
         o = Crash::o' ->
-        exec u o d s (Unseal h) (Crashed _ o' d s) []
+        exec st (Unseal h) (Crashed (u, o', d, s)) []
              
   | ExecRetCrash :
-      forall T u o d s o' (v: T),
+      forall st o' T (v: T),
+        let u := fst (fst (fst st)) in
+        let o := snd (fst (fst st)) in
+        let d := snd (fst st) in
+        let s := snd st in
         o = Crash::o' ->
-        exec u o d s (Ret v) (Crashed _ o' d s) []
+        exec st (Ret v) (Crashed (u, o', d, s)) []
              
   | ExecBindCrash :
       forall T T' (p1: prog T) (p2: T -> prog T')
-        u o d s o1 d1 s1 tr1,
-        exec u o d s p1 (Crashed _ o1 d1 s1) tr1 ->
-        exec u o d s (Bind p1 p2) (Crashed _ o1 d1 s1) tr1.
+        st st1 tr1,
+        exec st p1 (Crashed st1) tr1 ->
+        exec st (Bind p1 p2) (Crashed st1) tr1.
 
+
+  Inductive exec_lts :
+    forall T, state -> prog T -> @Result state T -> Prop :=
+  | Exec : 
+      forall T (p: prog T) st st' tr,
+        exec st p st' tr ->
+        exec_lts st p st'.
+
+  Definition prog_LTS := {| State:= state; Op:= prog; transition := exec_lts |}.
+  
+
+  Definition state_equivalent_for u (st1 st2: state) :=
+  let '(u1, o1, d1, s1) := st1 in
+  let '(u2, o2, d2, s2) := st2 in
+  u1 = u2 /\
+  o1 = o2 /\
+  @equivalent_for_fst _ addr_dec _ u d1 d2 /\
+  @equivalent_for _ handle_dec _ u s1 s2.
+
+  Definition return_equivalent_for {T} u (ret1 ret2: @Result state T) :=
+    match ret1, ret2 with
+    |Finished st1 r1, Finished st2 r2 =>
+     state_equivalent_for u st1 st2 /\ r1 = r2
+    |Crashed st1, Crashed st2 =>
+     state_equivalent_for u st1 st2
+    |_, _ => False
+    end.
+  
+  Definition return_state_equivalent_for {T} u (ret1 ret2: @Result state T) :=
+    match ret1, ret2 with
+    |Finished s1' _, Finished s2' _
+    |Crashed s1', Crashed s2' =>
+     state_equivalent_for u s1' s2'
+    | _, _ => False
+    end.
+  
+  Definition state_noninterference {T} (p: prog T) (valid: state -> Prop):=
+    forall viewer st1 st1' st2 tr,
+      valid st1 ->
+      (* valid st2 -> *)
+      exec st1 p st1' tr ->
+      state_equivalent_for viewer st1 st2 ->
+      exists st2' tr2,
+        exec st2 p st2' tr2 /\
+        return_state_equivalent_for viewer st1' st2'.
+
+  Definition ret_noninterference {T} (p: prog T) (valid: state -> Prop):=
+    forall st1 st1' st2 tr,
+      valid st1 ->
+      (* valid st2 -> *)
+      exec st1 p st1' tr ->
+      state_equivalent_for (get_user st1) st1 st2 ->
+    exists st2',
+      exec st2 p st2' tr /\
+      return_equivalent_for (get_user st1) st1' st2'.
+
+  Definition data_noninterference {T} (p: prog T) (valid: state -> Prop) :=
+    state_noninterference p valid /\
+    ret_noninterference p valid.
   
 End Prog.
 
