src/CommonAutomation.v
@@ -1,0 +1,114 @@
+Require Import BaseTypes Simulation.
+Require Import Memx.
+Require Import List.
+Require Import Eqdep.
+Import ListNotations.
+
+Tactic Notation "eapply_fresh" constr(thm) "in" hyp(H) :=
+  let Hx := fresh "Hx" in eapply thm in H as Hx.
+
+Tactic Notation "destruct_fresh" constr(term) :=
+  let D := fresh "D" in destruct term eqn:D.
+
+Tactic Notation "assert_fresh" constr(ass) :=
+  let A := fresh "A" in assert ass as A.
+
+Lemma app_cons_nil:
+  forall T (l: list T) a,
+    a::l = (a::nil)++l.
+Proof.
+  intros; simpl; auto.
+Qed.
+
+Lemma cons_app_inv_tail :
+  forall T (l l': list T) a,
+    a::l = l'++l ->
+    a::nil = l'.
+Proof.
+  intros.
+  rewrite app_cons_nil in H.
+  apply app_inv_tail in H; subst; auto.
+Qed.
+
+
+Ltac sigT_eq :=
+  match goal with
+  | [ H: existT ?P ?a _ = existT ?P ?a _ |- _ ] =>
+    apply Eqdep.EqdepTheory.inj_pair2 in H; subst; repeat sigT_eq
+  end.
+
+Ltac logic_clean:=
+  match goal with
+  | [H: exists _, _ |- _] => destruct H; repeat logic_clean
+  | [H: _ /\ _ |- _] => destruct H; repeat logic_clean
+  end.
+
+Ltac invert_const :=
+  match goal with
+  | [H: Some _ = Some _ |- _] => inversion H; subst; clear H; repeat invert_const
+  | [H: Some _ = None |- _] => inversion H
+  | [H: None = Some _ |- _] => inversion H
+  | [H: Finished _ _ = Finished _ _ |- _] => inversion H; subst; clear H; repeat invert_const
+  | [H: Crashed _ = Crashed _ |- _] => inversion H; subst; clear H; repeat invert_const
+  | [H: Finished _ _ = Crashed _ |- _] => inversion H
+  | [H: Crashed _ = Finished _ _ |- _] => inversion H
+  | [H: _ :: _ = _ :: _ |- _] => inversion H; subst; clear H; repeat invert_const
+  end.
+
+Ltac clear_dup:=
+  match goal with
+  | [H: ?x = ?x |- _] => clear H; repeat clear_dup
+  | [H: ?x, H0: ?x |- _] => clear H0; repeat clear_dup
+  end.
+
+Ltac rewrite_upd_eq:=
+  match goal with
+  |[H: upd _ ?x _ ?x = _ |- _] => rewrite upd_eq in H; repeat rewrite_upd_eq; try invert_const
+  end.
+
+Ltac rewriteall :=
+  match goal with
+  | [H := _ |- _] => subst H; repeat rewriteall
+  | [H: ?x = _, H0: ?x = _ |- _ ] => rewrite H in H0; repeat rewriteall
+  | [H: ?x = _, H0: _ = ?x |- _ ] => rewrite H in H0; repeat rewriteall
+  | [H: ?x = _ |- context [?x] ] => rewrite H; repeat rewriteall
+  end.
+
+
+Ltac clear_trace:=
+  match goal with
+  | [H: _++?tr = _++?tr |- _] =>
+    apply app_inv_tail in H; repeat clear_trace
+  | [H: ?tr = _++?tr |- _] =>
+    rewrite <- app_nil_l in H at 1; repeat clear_trace
+  | [H: _::?tr = _++?tr |- _] =>
+    apply cons_app_inv_tail in H; repeat clear_trace
+  | [H: _::_++?tr = _++?tr |- _] =>
+    rewrite app_comm_cons in H; repeat clear_trace
+  | [H: _++_++?tr = _++?tr |- _] =>
+    rewrite app_assoc in H; repeat clear_trace
+  | [H: _++?tr = _++_++?tr |- _] =>
+    rewrite app_assoc in H; repeat clear_trace
+  end.
+
+
+Ltac split_match:=
+  match goal with
+  |[H: context [match ?x with | _ => _ end] |- _] =>
+   let name := fresh "D" in
+     destruct x eqn:name; repeat split_match
+  end.
+
+Ltac cleanup:= try split_match; try logic_clean; subst; try rewriteall;
+               try clear_dup; try rewrite_upd_eq;
+               try clear_dup; try invert_const;
+               try clear_trace; try sigT_eq;
+               subst; try rewriteall.
+
+Ltac split_ors:=
+  match goal with
+  | [H: _ \/ _ |- _ ] => destruct H; cleanup
+  end.
+
+
+
