src/Layer2.v
@@ -1,0 +1,83 @@
+Require Import Primitives Simulation Confidentiality.
+Require Import SimpleDisk Omega FunctionalExtensionality.
+Require Import ProgLimited.
+Import ListNotations.
+Close Scope pred_scope.
+Set Implicit Arguments.
+
+Section Layer2.
+
+  Definition disk2 := @mem addr addr_dec sealed_value.
+  Definition state2 := (user * oracle * disk2 * store)%type.
+  Definition get_user (st: state2) := fst (fst (fst st)).
+  Definition get_oracle (st: state2) := snd (fst (fst st)).
+  Definition get_disk (st: state2) := snd (fst st).
+  Definition get_store (st: state2) := snd st.
+  
+  Inductive exec2 :
+    forall T, state2 -> prog_limited T -> @Result state2 T -> Prop :=
+  | Exec2Finished :
+      forall T (p: prog_limited T) u o d dh s o' d' dh' s' r,
+      exec_limited (u, o, d, s) p (Finished (u, o', d', s') r) ->
+      rep dh d ->
+      rep dh' d' ->
+      exec2 (u, o, dh, s) p (Finished (u, o', dh', s') r)
+  | Exec2Crashed :
+      forall T (p: prog_limited T) u o d dh s o' d' dh' s',
+      exec_limited (u, o, d, s) p (Crashed (u, o', d', s')) ->
+      rep dh d ->
+      rep dh' d' ->
+      exec2 (u, o, dh, s) p (Crashed (u, o', dh', s')).
+
+  Definition prog2_LTS := {| State:= state2; Op:= prog_limited; transition := exec2 |}.
+
+  Definition state_equivalent_for u (st1 st2: state2) :=
+  let '(u1, o1, d1, s1) := st1 in
+  let '(u2, o2, d2, s2) := st2 in
+  u1 = u2 /\
+  o1 = o2 /\
+  @equivalent_for _ addr_dec _ u d1 d2 /\
+  @equivalent_for _ handle_dec _ u s1 s2.
+
+  Definition return_equivalent_for {T} u (ret1 ret2: @Result state2 T) :=
+    match ret1, ret2 with
+    |Finished st1 r1, Finished st2 r2 =>
+     state_equivalent_for u st1 st2 /\ r1 = r2
+    |Crashed st1, Crashed st2 =>
+     state_equivalent_for u st1 st2
+    |_, _ => False
+    end.
+  
+  Definition return_state_equivalent_for {T} u (ret1 ret2: @Result state2 T) :=
+    match ret1, ret2 with
+    |Finished s1' _, Finished s2' _
+    |Crashed s1', Crashed s2' =>
+     state_equivalent_for u s1' s2'
+    | _, _ => False
+    end.
+  
+  Definition state_noninterference {T} (p: prog_limited T) (valid: state2 -> Prop):=
+  forall viewer st1 st1' st2,
+    valid st1 ->
+    valid st2 ->
+    exec2 st1 p st1' ->
+    state_equivalent_for viewer st1 st2 ->
+    exists st2',
+      exec2 st2 p st2' /\
+      return_state_equivalent_for viewer st1' st2'.
+
+  Definition ret_noninterference {T} (p: prog_limited T) (valid: state2 -> Prop) :=
+    forall st1 st1' st2,
+    valid st1 ->
+    valid st2 ->
+    exec2 st1 p st1' ->
+    state_equivalent_for (get_user st1) st1 st2 ->
+    exists st2',
+      exec2 st2 p st2' /\
+      return_equivalent_for (get_user st1) st1' st2'.
+
+  Definition data_noninterference {T} (p: prog_limited T) (valid: state2 -> Prop) :=
+    state_noninterference p valid /\
+    ret_noninterference p valid.
+
+End Layer2.
