src/LayerTransfer.v
@@ -1,0 +1,335 @@
+Require Import Primitives Simulation Confidentiality.
+Require Import SimpleDisk Omega FunctionalExtensionality.
+Require Import ProgLimited Layer2.
+Import ListNotations.
+Close Scope pred_scope.
+Set Implicit Arguments.
+
+
+Section LayerTransfer.
+
+  Definition right_total_filtered {T1 T2: Type} (R: T1 -> T2 -> Prop) (P: T2 -> Prop):=
+    forall t2,
+    P t2 ->
+    exists t1, R t1 t2.
+
+Definition simulation_preserving {T1 T2: Type} (S1: T1 -> T1 -> Prop) (S2: T2 -> T2 -> Prop)(R: T1 -> T2 -> Prop) :=
+  forall t1 t1' t2 t2',
+    R t1 t2 ->
+    R t1' t2' ->
+    S1 t1 t1' <-> S2 t2 t2'.
+    
+  Definition refines_to (s1 : state) (s2: state2) :=
+    Prog.get_user s1 = get_user s2 /\
+    Prog.get_oracle s1 = get_oracle s2 /\
+    rep (get_disk s2) (Prog.get_disk s1) /\
+    Prog.get_store s1 = get_store s2.
+
+  Ltac simpl_refines_to :=
+    unfold refines_to, Prog.get_user, get_user,
+        Prog.get_oracle, get_oracle,
+        Prog.get_disk, get_disk,
+        Prog.get_store, get_store in *; simpl in *.
+
+  
+  Ltac simpl_states:=
+    unfold state, state2 in *; destruct_pairs; simpl in *.
+
+  Definition refines_to_same st1 st2 := exists sr, refines_to st1 sr /\ refines_to st2 sr.
+
+
+  Lemma exec_preserves_user:
+      forall T (p: prog T) st1 st1' tr,
+        exec st1 p st1' tr ->
+        Prog.get_user st1 = Prog.get_user (extract_state st1').
+    Proof.
+      induction 1; simpl in *; eauto.
+      cleanup; eauto.
+    Qed.
+
+    Lemma exec_deterministic_oracle:
+      forall T (p: prog T) st1 st2 st1' st2' tr1 tr2,
+        exec st1 p st1' tr1 ->
+        exec st2 p st2' tr2 ->
+        Prog.get_oracle st1 = Prog.get_oracle st2 ->
+        Prog.get_oracle (extract_state st1') = Prog.get_oracle (extract_state st2').
+    Proof.
+      unfold Prog.get_oracle;
+        induction p; intros; simpl in *;
+          simpl_states; cleanup;
+            invert_exec; invert_exec;
+              cleanup; simpl in *;
+          cleanup; eauto;
+      try match goal with
+      |[H: _ :: _ = _ :: _ |- _] =>
+       inversion H; eauto
+          end.      
+      simpl_states; cleanup.
+   Abort.
+
+  
+  Lemma exec_limited_preserves_refinement:
+      forall T (p: prog_limited T)  st1 st2 st1' st2',
+        exec_limited st1 p st1' ->
+        exec_limited st2 p st2' ->
+        refines_to_same st1 st2 ->
+        refines_to_same (extract_state st1') (extract_state st2').
+  Proof.
+    unfold refines_to_same, refines_to;
+      induction p; simpl in *;
+        intros; simpl_refines_to; simpl_states; cleanup.
+    
+    - inversion H; sigT_eq; clear H;
+        inversion H0; sigT_eq; clear H0;
+          simpl_states.
+      edestruct alloc_ok; eauto.
+      apply pimpl_star_emp; eauto.
+      destruct H; cleanup.
+      destruct_lift H1.
+      edestruct alloc_ok; [| apply H6 | eauto].
+      apply pimpl_star_emp; eauto.
+      destruct H1; cleanup.
+      destruct_lift H3.
+      destruct H8, H11; cleanup.
+  Admitted.
+  
+  Lemma rep_equivalent_for:
+      forall u d1 d2 d1' d2',
+        equivalent_for_fst u d1 d1' ->
+        rep d2 d1 ->
+        rep d2' d1' ->
+        equivalent_for u d2 d2'.
+    Proof.
+      unfold equivalent_for, equivalent_for_fst, rep; intros.
+      destruct_lift H0; destruct_lift H1; cleanup.
+
+      specialize (H 0) as Hx; destruct Hx; cleanup.
+      erewrite ptsto_valid in H2; [| pred_apply; cancel]; cleanup.
+      
+      erewrite ptsto_valid in H2; [| pred_apply; cancel]; cleanup.
+      erewrite ptsto_valid in H3; [| pred_apply; cancel]; cleanup.
+      simpl in *; cleanup.
+      specialize (H18 (can_access_public u)); inversion H18; cleanup.
+
+      specialize (H a) as Hx.
+      
+      destruct (Compare_dec.le_lt_dec a 2); [|intuition].
+      destruct a; [intuition|].
+      destruct a.
+      destruct Hx; cleanup.
+      erewrite ptsto_valid in H2; [| pred_apply; cancel]; cleanup.
+      
+      erewrite ptsto_valid in H2; [| pred_apply; cancel]; cleanup.
+      erewrite ptsto_valid in H3; [| pred_apply; cancel]; cleanup.
+      simpl in *; cleanup.      
+      
+      destruct (value_to_nat dummy1); [intuition|].
+      destruct n; [intuition|].
+      right; do 2 eexists; intuition eauto; simpl in *.
+      destruct n; [intuition|].
+      destruct n; [intuition|].
+      right; do 2 eexists; intuition eauto; simpl in *.
+      omega.
+
+      destruct a; [|intuition].
+      destruct Hx; cleanup.
+      erewrite ptsto_valid in H2; [| pred_apply; cancel]; cleanup.
+      
+      erewrite ptsto_valid in H2; [| pred_apply; cancel]; cleanup.
+      erewrite ptsto_valid in H3; [| pred_apply; cancel]; cleanup.
+      simpl in *; cleanup.      
+      
+      destruct (value_to_nat dummy1); [intuition|].
+      destruct n; [intuition|].
+      destruct n; [intuition|].
+      right; do 2 eexists; intuition eauto; simpl in *.
+      destruct n; [intuition|].
+      right; do 2 eexists; intuition eauto; simpl in *.
+      omega.
+    Qed.
+
+    
+    Theorem RS_right_total_filtered :
+      right_total_filtered refines_to (fun d2 => exists d1, rep (get_disk d2) d1).
+    Proof.
+      unfold state, state2, refines_to, right_total_filtered; intros;
+      simpl_refines_to; simpl_states; cleanup.
+      exists (x, x0, x3, x2); destruct_pairs; intuition eauto.
+    Qed.
+
+    Lemma RS_simulation_preserving:
+      forall u, simulation_preserving refines_to_same (state_equivalent_for u) refines_to.
+    Proof.
+      unfold simulation_preserving, refines_to_same, refines_to,
+      Prog.state_equivalent_for, state_equivalent_for; intros.
+      simpl_refines_to; simpl_states; cleanup.
+      split; intros; cleanup; intuition.
+      admit.
+      admit.
+
+      exists(x, x0, x1, x2); intuition eauto.
+      simpl in *.
+    Abort.
+  
+    
+  
+
+    
+
+    Lemma exec_preserves_rep:
+      forall T (p: prog2 T)  st1 d1 st1' tr,
+        exec st1 (prog2_to_prog p) st1' tr ->
+        rep d1 (Prog.get_disk st1) ->
+        exists d1', rep d1' (Prog.get_disk (extract_state st1')).
+    Proof.
+      induction p; intros; cleanup; simpl in *; eauto;
+      unfold Prog.get_disk, state in *; destruct_pairs; simpl in *.
+      - edestruct alloc_ok; eauto.
+        apply pimpl_star_emp; eauto.
+        destruct H1; cleanup;
+        destruct_lift H3; eauto.
+
+      - edestruct free_ok; eauto.
+        apply pimpl_star_emp; eauto.
+        destruct H1; cleanup;
+        destruct_lift H3; eauto.
+
+      - edestruct read_ok; eauto.
+        apply pimpl_star_emp; eauto.
+        destruct H1; cleanup;
+        destruct_lift H3; eauto.
+
+      - edestruct write_ok'; eauto.
+        apply pimpl_star_emp; eauto.
+        destruct H1; cleanup;
+          destruct_lift H3; eauto.
+        
+      - invert_exec; cleanup; simpl in *; eauto.
+
+      - invert_exec.
+        eapply IHp in H0; eauto; cleanup; simpl in *.
+        eapply H in H2; eauto; cleanup; simpl in *.
+        
+        destruct H0; cleanup; simpl in *.
+        eapply IHp in H0; eauto; cleanup; simpl in *.
+        eapply IHp in H0; eauto; cleanup; simpl in *.
+        eapply H in H2; eauto; cleanup; simpl in *.
+    Qed.
+
+    
+
+    Theorem RS_strong_bisimulation:
+      StrongBisimulation prog_LTS prog2_LTS RP RS.
+    Proof.
+      unfold RP, RS; constructor; intros.
+      cleanup; simpl in *.
+      unfold Prog.get_user, get_user,
+        Prog.get_oracle, get_oracle,
+        Prog.get_disk, get_disk,
+        Prog.get_store, get_store in *; simpl in *; cleanup.
+      unfold state, state2 in *; destruct_pairs; simpl in *.
+      split; intros.
+
+      - inversion H; sigT_eq.
+        eapply_fresh exec_preserves_rep in H5; cleanup; simpl in *; eauto.
+        eapply_fresh exec_preserves_user in H5; simpl in *; cleanup.
+        destruct s1'; simpl in *; destruct_pairs; cleanup.
+        unfold Prog.get_user, Prog.get_disk in *; simpl in *; cleanup.
+        eexists; intuition.
+        econstructor; eauto.
+        all: simpl; eauto.
+
+        unfold Prog.get_user, Prog.get_disk in *; simpl in *; cleanup.
+        eexists; intuition.
+        eapply Exec2Crashed; simpl; eauto.
+        all: simpl; eauto.
+
+      - inversion H; sigT_eq.
+        simpl in *; eexists; intuition.
+    Abort.
+     *)
+
+    Theorem transfer_low_to_high_self :
+  forall T (p: prog2 T),
+   ->
+  StrongBisimulation prog_LTS prog2_LTS RP RS ->
+  (forall T, right_total (@RP T)) ->
+  right_total_filtered RS (fun d2 => exists d1, rep (get_disk d2) d1) ->
+  (forall u, simulation_preserving (Prog.state_equivalent_for u) (state_equivalent_for u) RS) ->
+  data_noninterference p (fun d2 => exists d1, rep (get_disk d2) d1).
+Proof.
+
+  Theorem transfer_low_to_high_self :
+  forall T (p: prog2 T),
+  Prog.data_noninterference (prog2_to_prog p) (fun d1 => exists d2, rep d2 (Prog.get_disk d1)) ->
+  StrongBisimulation prog_LTS prog2_LTS RP RS ->
+  (forall T, right_total (@RP T)) ->
+  right_total_filtered RS (fun d2 => exists d1, rep (get_disk d2) d1) ->
+  (forall u, simulation_preserving (Prog.state_equivalent_for u) (state_equivalent_for u) RS) ->
+  data_noninterference p (fun d2 => exists d1, rep (get_disk d2) d1).
+Proof.
+  unfold right_total, right_total_filtered, simulation_preserving, result_same; intros.
+  destruct H, H0.
+  rename H1 into right_total_op.
+  rename H2 into right_total_state.
+  rename H3 into simulation_preserving.
+
+  unfold data_noninterference; split.
+  - unfold state_noninterference; intros.
+    edestruct (right_total_state st1), (right_total_state st2); eauto.
+    edestruct (right_total_op T p).
+    eapply_fresh strong_bisimulation_correct0 in H5; eauto; cleanup; simpl in *.
+    apply H9 in H2; cleanup; clear H8 H9.
+
+    inversion H2; sigT_eq.
+    unfold Prog.state_noninterference, Prog.ret_noninterference in *.
+    unfold RP in *; cleanup.
+    eapply_fresh H in H15; eauto; cleanup.
+    eapply_fresh strong_bisimulation_correct0 in H6; eauto; cleanup; simpl in *.
+    edestruct H9; [econstructor; eauto|]; cleanup.
+    eexists; intuition eauto.
+    
+    unfold return_state_equivalent_for.
+    unfold result_same in *; cleanup; intuition eauto;
+    simpl in *;
+    unfold state_equivalent_for, Prog.state_equivalent_for in *; cleanup;
+    unfold RS in *; simpl in *;
+    unfold state, state2 in *; destruct_pairs; simpl in *; cleanup;
+    unfold Prog.get_user, get_user,
+    Prog.get_oracle, get_oracle,
+    Prog.get_disk, get_disk in *; simpl in *; cleanup;
+    intuition eauto; eapply rep_equivalent_for; eauto.
+
+    unfold RS in H5; cleanup; eauto.
+    eapply simulation_preserving; eauto.
+
+  -  unfold ret_noninterference; intros.
+     edestruct (right_total_state st1), (right_total_state st2); eauto.
+     edestruct (right_total_op T p).
+     eapply_fresh strong_bisimulation_correct0 in H5; eauto; cleanup; simpl in *.
+     apply H9 in H2; cleanup; clear H8 H9.
+     
+     inversion H2; sigT_eq.
+     unfold RP in *; cleanup.
+     unfold Prog.state_noninterference, Prog.ret_noninterference in *.
+     eapply_fresh H4 in H15; eauto; cleanup.
+     eapply_fresh strong_bisimulation_correct0 in H6; eauto; cleanup; simpl in *.     
+     edestruct H9; [econstructor; eauto|]; cleanup.
+     eexists; intuition eauto.
+     
+     unfold return_equivalent_for.
+     unfold result_same in *; cleanup; intuition eauto;
+       simpl in *;
+       unfold state_equivalent_for, Prog.state_equivalent_for in *; cleanup;
+         unfold RS in *; simpl in *;
+           unfold state, state2 in *; destruct_pairs; simpl in *; cleanup;
+             unfold Prog.get_user, get_user,
+             Prog.get_oracle, get_oracle,
+             Prog.get_disk, get_disk in *; simpl in *; cleanup;
+               intuition eauto; try eapply rep_equivalent_for; eauto.
+     
+     cleanup; eauto.
+     unfold RS in H5; simpl in *; cleanup; eauto.
+     pose proof H5 as Hx; unfold RS in H5; simpl in *; cleanup; eauto.
+     eapply simulation_preserving; eauto.
+Qed.
