src/Primitives.v
@@ -1,4 +1,4 @@
 Require Export List BaseTypes Memx Predx SepAuto.
-Require Export Disk Prog ProgAuto Hoare.
-Require Export OpSpec.
+Require Export Disk Simulation Prog ProgAuto Hoare.
+Require Export OpSpec CommonAutomation.
 Export ListNotations.
