src/ProgAuto.v
@@ -1,158 +1,62 @@
-Require Import BaseTypes Prog.
-Require Import Memx.
+Require Import BaseTypes Prog Simulation.
+Require Import Memx CommonAutomation.
 Require Import List.
 Require Import Eqdep.
 Import ListNotations.
 
-Lemma app_cons_nil:
-  forall T (l: list T) a,
-    a::l = (a::nil)++l.
-Proof.
-  intros; simpl; auto.
-Qed.
-
-Lemma cons_app_inv_tail :
-  forall T (l l': list T) a,
-    a::l = l'++l ->
-    a::nil = l'.
-Proof.
-  intros.
-  rewrite app_cons_nil in H.
-  apply app_inv_tail in H; subst; auto.
-Qed.
-
-
-Ltac sigT_eq :=
-  match goal with
-  | [ H: existT ?P ?a _ = existT ?P ?a _ |- _ ] =>
-    apply Eqdep.EqdepTheory.inj_pair2 in H; subst; repeat sigT_eq
-  end.
-
-
-Ltac inv_exec'' H :=
+Ltac invert_exec'' H :=
   inversion H; subst; clear H; repeat sigT_eq.
 
-Ltac inv_exec' :=
+Ltac invert_exec' :=
   match goal with
-  | [ H: exec _ _ _ _ (Ret _) _ _ |- _ ] =>
-    inv_exec'' H
-  | [ H: exec _ _ _ _ (Read _) _ _ |- _ ] =>
-    inv_exec'' H
-  | [ H: exec _ _ _ _ (Write _ _) _ _ |- _ ] =>
-    inv_exec'' H
-  | [ H: exec _ _ _ _ (Seal _ _) _ _ |- _ ] =>
-    inv_exec'' H
-  | [ H: exec _ _ _ _ (Unseal _) _ _ |- _ ] =>
-    inv_exec'' H
-  | [ H: exec _ _ _ _ (Auth _) _ _ |- _ ] =>
-    inv_exec'' H
+  | [ H: exec _ (Ret _) _ _ |- _ ] =>
+    invert_exec'' H
+  | [ H: exec _ (Read _) _ _ |- _ ] =>
+    invert_exec'' H
+  | [ H: exec _ (Write _ _) _ _ |- _ ] =>
+    invert_exec'' H
+  | [ H: exec _ (Seal _ _) _ _ |- _ ] =>
+    invert_exec'' H
+  | [ H: exec _ (Unseal _) _ _ |- _ ] =>
+    invert_exec'' H
+  | [ H: exec _ (Auth _) _ _ |- _ ] =>
+    invert_exec'' H
   end.
 
 Lemma bind_sep:
-  forall T T' pr (p1: prog T) (p2: T -> prog T') d bm dm (ret: result T') tr',
-    exec pr d bm dm (Bind p1 p2) ret tr' ->
+  forall T T' st (p1: prog T) (p2: T -> prog T') ret tr',
+    exec st (Bind p1 p2) ret tr' ->
     match ret with
-    | Finished _ _ _ _ =>
-    (exists tr1 tr2 r1 d1 dm1 bm1,
-       exec pr d bm dm p1 (Finished d1 bm1 dm1 r1) tr1 /\
-       exec pr d1 bm1 dm1 (p2 r1) ret tr2 /\ tr' = tr1 ++ tr2)
-  | Crashed _ d' bm' dm' =>
-    (exec pr d bm dm p1 (Crashed _ d' bm' dm') tr' \/
-     (exists tr1 tr2 r1 d1 dm1 bm1,
-        exec pr d bm dm p1 (Finished d1 bm1 dm1 r1) tr1 /\
-        exec pr d1 bm1 dm1 (p2 r1) ret tr2 /\ tr' = tr1 ++ tr2))
+    | Finished st' r =>
+    (exists tr1 tr2 r1 st1,
+       exec st p1 (Finished st1 r1) tr1 /\
+       exec st1 (p2 r1) ret tr2 /\ tr' = tr1 ++ tr2)
+  | Crashed st' =>
+    (exec st p1 (Crashed st') tr' \/
+     (exists tr1 tr2 r1 st1,
+        exec st p1 (Finished st1 r1) tr1 /\
+        exec st1 (p2 r1) ret tr2 /\ tr' = tr1 ++ tr2))
     end.
 Proof.
   intros.
-  inv_exec'' H; eauto.
+  invert_exec'' H; eauto.
   destruct ret.
-  do 7 eexists; eauto.
-  right; do 7 eexists; eauto.
+  do 4 eexists; eauto.
+  right; do 4 eexists; eauto.
 Qed.
 
-Ltac logic_clean:=
+Ltac invert_exec :=
   match goal with
-  | [H: exists _, _ |- _] => destruct H; repeat logic_clean
-  | [H: _ /\ _ |- _] => destruct H; repeat logic_clean
-  end.
-
-Ltac invert_const :=
-  match goal with
-  | [H: Some _ = Some _ |- _] => inversion H; subst; clear H; repeat invert_const
-  | [H: Some _ = None |- _] => inversion H
-  | [H: None = Some _ |- _] => inversion H
-  | [H: Finished _ _ _ _ = Finished _ _ _ _ |- _] => inversion H; subst; clear H; repeat invert_const
-  | [H: Crashed _ _ _ _ = Crashed _ _ _ _ |- _] => inversion H; subst; clear H; repeat invert_const
-  | [H: Finished _ _ _ _ = Crashed _ _ _ _ |- _] => inversion H
-  | [H: Crashed _ _ _ _ = Finished _ _ _ _ |- _] => inversion H
-  | [H: _ :: _ = _ :: _ |- _] => inversion H; subst; clear H; repeat invert_const
-  end.
-
-Ltac clear_dup:=
-  match goal with
-  | [H: ?x = ?x |- _] => clear H; repeat clear_dup
-  | [H: ?x, H0: ?x |- _] => clear H0; repeat clear_dup
-  end.
-
-Ltac rewrite_upd_eq:=
-  match goal with
-  |[H: upd _ ?x _ ?x = _ |- _] => rewrite upd_eq in H; repeat rewrite_upd_eq; try invert_const
-  end.
-
-Ltac rewriteall :=
-  match goal with
-  | [H: ?x = _, H0: ?x = _ |- _ ] => rewrite H in H0; repeat rewriteall
-  | [H: ?x = _, H0: _ = ?x |- _ ] => rewrite H in H0; repeat rewriteall
-  | [H: ?x = _ |- context [?x] ] => rewrite H; repeat rewriteall
-  end.
-
-
-Ltac clear_trace:=
-  match goal with
-  | [H: _++?tr = _++?tr |- _] =>
-    apply app_inv_tail in H; repeat clear_trace
-  | [H: ?tr = _++?tr |- _] =>
-    rewrite <- app_nil_l in H at 1; repeat clear_trace
-  | [H: _::?tr = _++?tr |- _] =>
-    apply cons_app_inv_tail in H; repeat clear_trace
-  | [H: _::_++?tr = _++?tr |- _] =>
-    rewrite app_comm_cons in H; repeat clear_trace
-  | [H: _++_++?tr = _++?tr |- _] =>
-    rewrite app_assoc in H; repeat clear_trace
-  | [H: _++?tr = _++_++?tr |- _] =>
-    rewrite app_assoc in H; repeat clear_trace
-  end.
-
-
-Ltac split_match:=
-  match goal with
-  |[H: context [match ?x with | _ => _ end] |- _] =>
-   let name := fresh "D" in
-     destruct x eqn:name; repeat split_match
-  end.
-
-Ltac cleanup:= try split_match; try logic_clean; subst; try rewriteall;
-               try clear_dup; try rewrite_upd_eq;
-               try clear_dup; try invert_const;
-               try clear_trace; try sigT_eq;
-               subst; try rewriteall.
-
-Ltac split_ors:=
-  match goal with
-  | [H: _ \/ _ |- _ ] => destruct H; cleanup
-  end.
-
-
-Ltac inv_exec_perm :=
-  match goal with
-  |[H : exec _ _ _ _ (Bind _ _) _ _ |- _ ] => apply bind_sep in H; repeat cleanup
-  |[H : exec _ _ _ _ _ _ _ |- _ ] => inv_exec'
+  |[H : exec _ (Bind _ _) _ _ |- _ ] =>
+   apply bind_sep in H; repeat cleanup
+  |[H : exec _ _ _ _ |- _ ] =>
+   invert_exec'
   end.
 
 
   Definition prog_equiv T : prog T -> prog T -> Prop :=
-    fun p1 p2 => forall pr d bm dm tr' out,
-        exec pr d bm dm p1 out tr' <-> exec pr d bm dm p2 out tr'.
+    fun p1 p2 => forall st tr' out,
+        exec st p1 out tr' <-> exec st p2 out tr'.
 
   Arguments prog_equiv {T} _ _.
 
@@ -162,27 +66,27 @@ Ltac inv_exec_perm :=
       Bind (Bind p1 p2) p3 ~= Bind p1 (fun x => Bind (p2 x) p3).
   Proof.
     split; intros.
-    - repeat inv_exec_perm; cleanup.
+    - repeat invert_exec; cleanup.
       rewrite <- app_assoc.
       repeat econstructor; eauto.
 
       split_ors.
-      inv_exec_perm; cleanup.
+      invert_exec; cleanup.
       split_ors; cleanup.
       eapply ExecBindCrash; auto.      
       econstructor; eauto.
       eapply ExecBindCrash; eauto.
-      inv_exec_perm.
+      invert_exec.
       rewrite <- app_assoc.
       repeat econstructor; eauto.
     
-    - repeat inv_exec_perm; cleanup.
+    - repeat invert_exec; cleanup.
       rewrite app_assoc.
       repeat (eapply ExecBind; eauto).
       
       split_ors.
       repeat econstructor; eauto.
-      inv_exec_perm.
+      invert_exec.
       split_ors.
       eapply ExecBindCrash; eauto.
       econstructor; eauto.
