src/ProgLimited.v
@@ -1,0 +1,61 @@
+Require Import Primitives Simulation Confidentiality.
+Require Import SimpleDisk Omega FunctionalExtensionality.
+Import ListNotations.
+Close Scope pred_scope.
+Set Implicit Arguments.
+
+Section ProgLimited.
+
+  Inductive prog_limited : Type -> Type :=
+  | Alloc : prog_limited (option addr)
+  | Free : addr -> prog_limited unit
+  | Read : addr -> prog_limited (option handle)
+  | Write : addr -> handle -> prog_limited (option unit)
+  | Ret : forall T, T -> prog_limited T
+  | Bind : forall T T', prog_limited T -> (T -> prog_limited T') -> prog_limited T'.
+
+  Fixpoint prog_limited_to_prog {T} (p: prog_limited T) : prog T :=
+    match p with
+    | Alloc => alloc
+    | Free a => free a
+    | Read a => read a
+    | Write a h => write a h
+    | Ret v => Prog.Ret v
+    | Bind p1 p2 => Prog.Bind (prog_limited_to_prog p1) (fun x => prog_limited_to_prog (p2 x))
+    end.
+  
+  Inductive exec_limited :
+    forall T, state -> prog_limited T -> @Result state T -> Prop :=
+  | ExecLimited :
+      forall T (p: prog_limited T) st1 st2 tr,
+      exec st1 (prog_limited_to_prog p) st2 tr ->
+      exec_limited st1 p st2.
+
+  Definition prog2_LTS := {| State:= state; Op:= prog_limited; transition := exec_limited |}.
+  
+  Definition state_noninterference {T} (p: prog_limited T) (valid: state -> Prop):=
+  forall viewer st1 st1' st2,
+    valid st1 ->
+    valid st2 ->
+    exec_limited st1 p st1' ->
+    state_equivalent_for viewer st1 st2 ->
+    exists st2',
+      exec_limited st2 p st2' /\
+      return_state_equivalent_for viewer st1' st2'.
+
+  Definition ret_noninterference {T} (p: prog_limited T) (valid: state -> Prop) :=
+    forall st1 st1' st2,
+    valid st1 ->
+    valid st2 ->
+    exec_limited st1 p st1' ->
+    state_equivalent_for (get_user st1) st1 st2 ->
+    exists st2',
+      exec_limited st2 p st2' /\
+      return_equivalent_for (get_user st1) st1' st2'.
+
+  Definition data_noninterference {T} (p: prog_limited T) (valid: state -> Prop) :=
+    state_noninterference p valid /\
+    ret_noninterference p valid.
+  
+End ProgLimited.
+
