src/SimulationV2.v
@@ -1,0 +1,61 @@
+Require Import List.
+
+Record ParametricEquivalence (P: Type) (T: Type) :=
+  {
+    eq : P -> T -> T -> Prop;
+    
+    eq_refl: forall p t, eq p t t;
+    eq_sym: forall p t t', eq p t t' -> eq p t' t;
+    eq_trans: forall p t t' t'', eq p t t' -> eq p t' t'' -> eq p t t'';
+  }.
+
+Inductive Result {State T: Type} :=
+| Finished : State -> T -> @Result State T
+| Crashed : State -> @Result State T.
+
+Definition extract_state {State T} (res: @Result State T) :=
+  match res with
+  | Finished s _ | Crashed s => s
+  end.
+
+Definition extract_ret {State T} def (res: @Result State T) :=
+  match res with
+  | Finished _ r => r
+  | Crashed _ => def
+  end.
+
+Definition map_state {State1 State2 T} (f:State1 -> State2) (res: @Result State1 T) :=
+  match res with
+  | Finished s v => Finished (f s) v
+  | Crashed s => Crashed (f s)
+  end.
+
+Lemma extract_state_map_state_elim:
+  forall ST1 ST2 T (R:ST1 -> ST2) (r : @Result ST1 T),
+    extract_state (map_state R r) = R (extract_state r).
+Proof.
+  intros; destruct r; simpl; eauto.
+Qed.
+
+Lemma extract_ret_map_state_elim:
+  forall ST1 ST2 T (R:ST1 -> ST2) (r : @Result ST1 T) def,
+    extract_ret def (map_state R r) = extract_ret def r.
+Proof.
+  intros; destruct r; simpl; eauto.
+Qed.
+
+Definition result_same {State1 State2 T1 T2} (res1: @Result State1 T1) (res2: @Result State2 T2) :=
+  match res1, res2 with
+  | Finished _ _, Finished _ _ | Crashed _, Crashed _ => True
+  | _, _ => False
+  end.
+
+Record Layer :=
+  {
+    State : Type;
+    Valid : State -> Prop;
+    Prog : Type -> Type;
+    Exec : forall T, State -> Prog T -> @Result State T -> Prop;
+    State_Equivalent : forall T, ParametricEquivalence T State;
+    Result_Equivalent : forall T T', ParametricEquivalence T (@Result State T')
+  }.
