Makefile
@@ -4,12 +4,13 @@ TEST_VFILES := $(shell find 'src' -name "*Tests.v")
 PROJ_VFILES := $(shell find 'src' -name "*.v")
 VFILES := $(filter-out $(TEST_VFILES),$(PROJ_VFILES))
 
-COQARGS :=
+COQARGS := 
 
 default: $(VFILES:.v=.vo)
 test: $(TEST_VFILES:.v=.vo) $(VFILES:.v=.vo)
 
 _CoqProject: libname $(wildcard vendor/*)
+	@echo "-quick" > $@
 	@echo "-R src $$(cat libname)" > $@
 	@for libdir in $(wildcard vendor/*); do \
 	libname=$$(cat $$libdir/libname); \
